%=======================================================================
\subsection{Quadratic action for phonons}
%======================================================================
%
In this section we use the expansions \eqref{eq:expansions_b_y_u} to expand the action \eqref{eq:eft_action_exact} up to second order in phonon fields $\pi^\alpha \pi^\beta$ and mixed order in metric perturbations $h_{\mu\nu}\,\pi^\alpha$.
To get some intuition we first present the flat-spacetime case, since formulas are cleaner and  ultimately exact in the limit $\rho/ M_{Pl}^{4}\to0$.

%-----------------------------------------------------------------
\subsubsection{Quadratic action in flat spacetime}
%-------------------------------------------------------
%
We refer to the full computations in curved spacetime below not to repeat the same steps.
In flat spacetime $a=1$ and $h_{\mu\nu}=0$, only the first terms in the action \eqref{eq:final_quadratic_action_curved_spacetime} survive, and we can integrate by parts in both space and time the term $\partial_j \pi^0\dot{\pi}^j = -\dot{\pi}^0(\partial_j \pi^j)$ to get
{\small\begin{align}
\begin{aligned}
    S^{(2)}&= \int d^4x \frac{(yF_y-bF_b)}{2}\bigg\{(\dot{\pi}^i)^2 - (\partial_j\pi^j)^2\Big[-\frac{b^2F_{bb}}{(yF_y-bF_b)}\Big]\\
    &\qquad\qquad\qquad\qquad\qquad+(\dot{\pi}^0)^2 \frac{y^2F_{yy}}{(yF_y-bF_b)}
    - 2\dot{\pi}^0 (\partial_j \pi^j) \frac{(yF_y-byF_{by})}{(yF_y-bF_b)}
    \bigg\}\\
    &=\int d^4x \frac{(\rho+p)}{2}\bigg\{(\dot{\pi}^i)^2 - \mathcal{C} (\partial_j\pi^j)^2 
    + (\dot{\pi}^0)^2 \mathcal{A}
    - 2\mathcal{M}\dot{\pi}^0 (\partial_j \pi^j) 
    \bigg\}
\end{aligned}
\end{align}}
for $\rho= -F + y F_y$, $p= F - b F_b$ and 
{\small\begin{align}
\begin{aligned}
    &\mathcal{C} = -\frac{b^2F_{bb}}{(yF_y-bF_b)},\quad 
    \mathcal{A} = \frac{y^2F_{yy}}{(yF_y-bF_b)} = \frac{T\, \frac{\partial\rho }{\partial T}}{\rho+p},\quad
    \mathcal{M} = \frac{(yF_y-byF_{by})}{(yF_y-bF_b)}.
\end{aligned}
\end{align}}
The entropy field $\pi^0$ is thus non-dynamical and the resulting constraint equation gives
\begin{align}
    \dot{\pi}^0 = \frac{\mathcal{M}}{\mathcal{A}} (\partial_j \pi^j) + \text{const.}
\end{align}
The constant is not physical and is reabsorbed in the factor $\gamma$ of the original definition $\varphi^0:=\gamma(t+\pi^0)$.
After solving the constraint, the action for the coordinate $\pi^i$ becomes
{\small
\begin{align}
    S^{(2)}&= \int d^4x \frac{(\rho+p)}{2}\Big[(\dot{\pi}^i)^2 - c_s^2 (\partial_j\pi^j)^2 \Big], \quad \text{for}\quad c_s^2 = \mathcal{C} + \frac{\mathcal{M}^2}{\mathcal{A}}.
\end{align}
}
We note the entropy contribution to the speed of sound is always positive in \emph{physical} situations.
Indeed $\mathcal{M}^2$ is a true square and, recalling $y\equiv T$, we have
\begin{equation}
    \mathcal{A}= \frac{T\, \frac{\partial\rho }{\partial T}}{\rho+p}\geq 0 \quad\text{provided}\quad
    \begin{cases}
        \rho+p\geq 0 \quad(\text{no ghosts}),\\
        \frac{\partial\rho }{\partial T} \geq 0 \quad(\text{positive heat capacity}).
    \end{cases} 
\end{equation}
Finally we confirm the speed of sound $c_s^2$, defined as the coefficient of the gradient term for the fluctuations above, always matches the thermodynamical definition of \emph{adiabatic} sound speed \eqref{eq:adiabatic_cs_nonadiabatic_pressure}, namely
\begin{align}\label{eq:cs_equiv_ca_flat_spacetime}
    c_a^2:= \frac{\partial p}{\partial \rho}_{\mid \sigma} \overset{\text{proved before}}{=}\frac{-b^2F_{bb} F_{yy}+(F_y-bF_{yb})^2}{F_{yy}\,(yF_y-bF_b)} \overset{\text{easy check}}{\equiv} c_s^2.
\end{align}
This is expected: longitudinal phonons, i.e. sound waves, do propagate with the speed of sound!





%-----------------------------------------------------------------
\subsubsection{Quadratic action in curved spacetime {\color{red}(in progress)}}
%--------------------------------------------------------------
%
{\color{red}[I am reporting the full computation here since I am not yet satisfied with the final form. It will eventually be moved to the computation appendix.]}\todotag{Read \& feel the struggle}

\noindent
We now consider a general perturbed FRW metric written as in \eqref{eq:general_perturbed_FLRW_metric} and expand the action up to quadratic order  $\pi^\alpha \pi^\beta,\,h_{\mu\nu}\,\pi^\alpha$ for fluid perturbations
{\small\begin{align}
\begin{aligned}
    S&=\int d^4x \sqrt{-g} F(b,y) = \int d^4x\,a^4 \big[1+\tfrac12 (h^{ii}-h^{00}) \big] F(\bar{b}(1+\delta b), \bar{y}(1+\delta y))
    \\
    &= \int \!\!\!d^4\!x\, a^4 \!\big[1+\tfrac12 (h^{ii}-h^{00}) \big]
    \Bigg[ F(\bar{b}, \bar{y}) + (\bar{b}F_b)  (\delta b^{(1)} + \delta b^{(2)}) + (\bar{y}F_y) (\delta y^{(1)} + \delta y^{(2)})\\
    &\,\,\qquad\qquad\qquad\qquad\qquad\qquad+ \tfrac12 (\bar{b}^2 F_{bb})(\delta b^{(1)})^2 + \tfrac12 (\bar{y}^2 F_{yy}) (\delta y^{(1)})^2
    + (\bar{b}\bar{y} F_{by}) \delta b^{(1)} \delta y^{(1)} \Bigg]
\end{aligned}
\end{align}}
Inserting the expansions \eqref{eq:expansions_b_y_u} for $b$ and $y$, the quadratic part of the action is then
{\small\begin{align}
\begin{aligned}
    S^{(2)}&=\int d^4x\,\, a^4 \bigg\{
        (\bar{b}F_b) (h^{ii}-h^{00}) \Big[(\partial_j \pi^j) - \tfrac12 h^{ii}\Big]
        + (\bar{y}F_y) (h^{ii}-h^{00}) \Big[\tfrac12 h^{00}+ \dot{\pi}^0\Big]\\
    &\quad + (\bar{b}F_b) \Big[ - h^{0 i} \dot{\pi}^i - \tfrac12  h^{ii} (\partial_j \pi^j) - \tfrac12 (\dot{\pi}^i)^2 + \tfrac12 (\partial_j \pi^j)^2 -\tfrac12 \partial_i\pi^j\partial_j\pi^i\Big]
    \\
    &\quad + (\bar{y}F_y) \Big[ \tfrac12 h^{00}\dot{\pi}^0+ h^{0 i} \dot{\pi}^i + \tfrac12 (\dot{\pi}^i)^2 -\partial_j\pi^0\dot{\pi}^j\Big]
    + \tfrac12 (\bar{b}^2 F_{bb})\Big[ (\partial_j \pi^j) - \tfrac12 h^{ii}\Big]^2
    \\
    &\quad + \tfrac12 (\bar{y}^2 F_{yy})\Big[\tfrac12 h^{00}+ \dot{\pi}^0\Big]^2
    + (\bar{b}\bar{y} F_{by}) \Big[(\partial_j \pi^j) - \tfrac12 h^{ii}\Big]\Big[\tfrac12 h^{00}+ \dot{\pi}^0\Big]
        \bigg\}.
\end{aligned}
\end{align}}
Dropping  further second orders in metric perturbations and {\color{blue} integrating by parts in space}\footnote{\label{fn:integrating_parts_space_backround}Space derivatives yield no further terms since the background isspatially homogenous.}, we get
{\small\begin{align}
\begin{aligned}
    S^{(2)}=
    \int d^4x\,\, a^4 \bigg\{&
        (\bar{b}F_b) (h^{ii}-h^{00}) (\partial_j \pi^j)
        + (\bar{y}F_y) (h^{ii}-h^{00}) \dot{\pi}^0 \\
    &\quad + (\bar{b}F_b) \Big[ - h^{0 i} \dot{\pi}^i - \tfrac12  h^{ii} (\partial_j \pi^j) - \tfrac12 (\dot{\pi}^i)^2 + \bluecancel{\tfrac12 (\partial_j \pi^j)^2} -\bluecancel{\tfrac12 \partial_i\pi^j\partial_j\pi^i}\Big]
    \\
    &\quad + (\bar{y}F_y) \Big[ \tfrac12 h^{00}\dot{\pi}^0+ h^{0 i} \dot{\pi}^i + \tfrac12 (\dot{\pi}^i)^2 -\partial_j\pi^0\dot{\pi}^j\Big]
    \\
    &\quad + \tfrac12 (\bar{b}^2 F_{bb})\Big[ (\partial_j \pi^j)^2 - h^{ii}(\partial_j \pi^j)\Big]
    + \tfrac12 (\bar{y}^2 F_{yy})\Big[h^{00} \dot{\pi}^0+ (\dot{\pi}^0)^2\Big]\\
    &\quad+ (\bar{b}\bar{y} F_{by}) \Big[ \dot{\pi}^0(\partial_j \pi^j) - \tfrac12 h^{ii}\dot{\pi}^0 + \tfrac12 h^{00} (\partial_j\pi^j)\Big]
        \bigg\}.
\end{aligned}
\end{align}}
Collecting terms $\pi^\alpha\pi^\beta$ and $\pi^\alpha h_{\mu\nu}$, the final expression for the quadratic action is then
{\small\begin{align}\label{eq:final_quadratic_action_curved_spacetime}
\begin{aligned}
    S^{(2)}=
    &\int d^4x\,\,a^4\,\,\bigg\{
    \tfrac12 (yF_y-bF_b) (\dot{\pi}^i)^2+\tfrac12 b^2 F_{bb} (\partial_j \pi^j)^2
    +\tfrac12 y^2 F_{yy} (\dot{\pi}^0)^2 \\
    &\qquad\qquad\qquad+ (b y F_{by}) (\dot{\pi}^0 \partial_j \pi^j)-(yF_y) (\partial_j \pi^0\dot{\pi}^j)
    \bigg\}\\
    &\quad + a^4\,\,\bigg\{
    \tfrac12\!\left(\bar{b}F_b - \bar{b}^2 F_{bb}\right) h^{ii}(\partial_j \pi^j)
    + \tfrac12\!\left(-2\bar{b}F_b + \bar{b}\bar{y}F_{by}\right) h^{00}(\partial_j \pi^j)\\
    &\qquad\qquad+ \left(\bar{y}F_y - \bar{b}F_b\right) h^{0j}\,\dot{\pi}^j + \tfrac12\!\left(2\bar{y}F_y - \bar{b}\bar{y}F_{by}\right) h^{ii}\dot{\pi}^0
    + \tfrac12\!\left(\bar{y}^2 F_{yy} - \bar{y}F_y\right) h^{00}\dot{\pi}^0
    \bigg\}\,.
\end{aligned}
\end{align}}
Note that only \emph{longitudinal} modes $\pi^j_{||}\propto\, \partial_j\pi^j$ are dynamical.
Transverse modes $\pi^j_{\perp}$ simply mix with vector metric perturbations $h^{0j}$ with resulting equation of motion
{\small\begin{align}\label{eq:eom_transverse_phonons}
    a^4\,\big(\bar{\rho}+\bar{p}\big)\,\big(\dot{\pi}_\perp^j + h^{0j}\,\big)=\text{const}\,.
\end{align}}
This is expected since vorticity in the fluid sources vector modes in the metric and viceversa.

In the following we thus restrict to longitudinal modes $\pi_{||}^j$.
Gathering $\rho+p=yF_y-bF_b$ outside the brackets to highlight ghosts, we rewrite the action \eqref{eq:final_quadratic_action_curved_spacetime} as\todotag{Probably should wait and integrate bp first}
{\small\begin{align}
\begin{aligned}
    S^{(2)}= &\int d^4x\,\,a^4\, (\rho+p)\,\bigg\{
    \tfrac12 (\dot{\pi}^i)^2-\tfrac12 \underbrace{\tfrac{-b^2 F_{bb}}{(yF_y-bF_b)}}_{=\mathcal{C}} (\partial_j \pi^j)^2
    +\tfrac12 \underbrace{\tfrac{y^2 F_{yy}}{(yF_y-bF_b)}}_{=\mathcal{A}} (\dot{\pi}^0)^2 \\
    &\quad\qquad\qquad\qquad\qquad+ \tfrac{(b y F_{by})}{(yF_y-bF_b)} (\dot{\pi}^0 \partial_j \pi^j)-\tfrac{(yF_y)}{(yF_y-bF_b)} (\partial_j \pi^0\dot{\pi}^j)
    \bigg\}\\
    & \,\,+ a^4\, (\rho+p)\, \bigg\{
    \tfrac12\!\left(\tfrac{\bar{b}F_b - \bar{b}^2 F_{bb}}{(yF_y-bF_b)}\right) h^{ii}(\partial_j \pi^j)
    + \tfrac12\!\left(\tfrac{-2\bar{b}F_b + \bar{b}\bar{y}F_{by}}{(yF_y-bF_b)}\right) h^{00}(\partial_j \pi^j)\\
    &\quad\qquad\qquad+ \left(\tfrac{\bar{y}F_y - \bar{b}F_b}{(yF_y-bF_b)}\right) h^{0 j}\,\dot{\pi}^j + \tfrac12\!\left(\tfrac{2\bar{y}F_y - \bar{b}\bar{y}F_{by}}{(yF_y-bF_b)}\right) h^{ii}\dot{\pi}^0
    + \tfrac12\!\left(\tfrac{\bar{y}^2 F_{yy} - \bar{y}F_y}{(yF_y-bF_b)}\right) h^{00}\dot{\pi}^0
    \bigg\}.
\end{aligned}
\end{align}}
%
Integrating by parts in both time and space the term $\partial_j \pi^0\dot{\pi}^j$ we get\footnotemark[\getrefnumber{fn:integrating_parts_space_backround}]
{\small
\begin{align}
\begin{aligned}
    S^{(2)}&=\int d^4x\, -(\partial_j \pi^j\, \pi^{0})\tfrac{d}{d\tau}(a^4yF_y)\\
    &+a^4\,\bigg\{
    \tfrac12 (yF_y-bF_b) (\dot{\pi}^i)^2+ \tfrac12 b^2 F_{bb} (\partial_j \pi^j)^2 +\tfrac12 y^2 F_{yy} (\dot{\pi}^0)^2+(b y F_{by}-yF_y) (\dot{\pi}^0 \partial_j \pi^j)\bigg\}\\
    &+ a^4\,\,\bigg\{
    \tfrac12\!\left(\bar{b}F_b - \bar{b}^2 F_{bb}\right) h^{ii}(\partial_j \pi^j)
    + \tfrac12\!\left(-2\bar{b}F_b + \bar{b}\bar{y}F_{by}\right) h^{00}(\partial_j \pi^j)+\left(\bar{y}F_y - \bar{b}F_b\right) h^{0 j}\,\dot{\pi}^j\\
    &\qquad\qquad +\tfrac12\!\left(2\bar{y}F_y - \bar{b}\bar{y}F_{by}\right) h^{ii}\dot{\pi}^0
    + \tfrac12\!\left(\bar{y}^2 F_{yy} - \bar{y}F_y\right) h^{00}\dot{\pi}^0
    \bigg\}.
\end{aligned}
\end{align}}
%
The constraint equation for $\pi^0$ now reads
{\small\begin{align}
\begin{aligned}
    \frac{d}{d\tau}&a^4\bigg[y^2F_{yy}\dot{\pi}^0+(byF_{by}-yF_y) (\partial_j\pi^j)+\tfrac12\!\big(2{y}F_y - byF_{by}\big) h^{ii}
    + \tfrac12\!\left({y}^2 F_{yy} - {y}F_y\right) h^{00}\bigg]
    \\
    &=-(\partial_j \pi^j)\tfrac{d}{d\tau}(a^4yF_y)\,.
\end{aligned}
\end{align}}
Resolving the constraint and plugging it back into the action we get
{\small\begin{align}
\begin{aligned}
    S^{(2)}&=
    \int d^4x\,\, a^4\,\bigg\{
    \tfrac12 (yF_y-bF_b) (\dot{\pi}^i)^2+ \tfrac12 b^2 F_{bb} (\partial_j \pi^j)^2\bigg\} -\tfrac12 a^4 y^2F_{yy} (\dot{\pi}^0)^2\\
    & \,\,\,+ a^4\bigg\{\tfrac12\!\left(\bar{b}F_b - \bar{b}^2 F_{bb}\right) h^{ii}(\partial_j \pi^j)
    + \tfrac12\!\left(\bar{b}\bar{y}F_{by}-2\bar{b}F_b\right) h^{00}(\partial_j \pi^j)+\left(\bar{y}F_y - \bar{b}F_b\right) h^{0j}\,\dot{\pi}^j \bigg\},
\end{aligned}
\end{align}}
where now\todotag{2nd form likely better}
{\small
\begin{align}
\begin{aligned}
    a^4y^2F_{yy}\dot{\pi}^0
    =&-a^4\bigg[(byF_{by}-yF_y) (\partial_j\pi^j)+\tfrac12\!\big(2{y}F_y - byF_{by}\big) h^{ii}
    + \tfrac12\!\left({y}^2 F_{yy} - {y}F_y\right) h^{00}\bigg]\\
    &-\int d\tau\, (\partial_j \pi^j)\tfrac{d}{d\tau}(a^4yF_y)\\
    &{\color{red}=-a^4\bigg[(byF_{by}-yF_y) (\partial_j\pi^j)+\bigg(\tfrac{1}{a^4}\!\!\int d\tau(\partial_j \pi^j)\tfrac{d}{d\tau}(a^4yF_y)\bigg)\bigg]}\\
    &{\color{red}\qquad-a^4\tfrac12\Big[\big(2{y}F_y - byF_{by}\big) h^{ii}+ \left({y}^2 F_{yy} - {y}F_y\right) h^{00}\Big]}.
\end{aligned}
\end{align}}
That is
{\small
\begin{align}
\begin{aligned}
    -\tfrac12&a^4y^2F_{yy}\big(\dot{\pi}^0\big)^2\\
    &=-\tfrac12 a^4 \tfrac{(byF_{by}-yF_y)^2}{y^2F_{yy}} (\partial_j\pi^j)^2\\
    &\quad-\tfrac{(byF_{by}-yF_y)}{y^2F_{yy}} (\partial_j\pi^j)\bigg(\int(\partial_\ell\pi^\ell)\tfrac{d}{d\tau}(a^4yF_y) \bigg)
    -\tfrac12 \tfrac{a^{-4}}{y^2F_{yy}}\bigg(\int(\partial_\ell\pi^\ell)\tfrac{d}{d\tau}(a^4yF_y)\bigg)^2
    \\
    &\quad-\tfrac12 a^4\tfrac{\big(2{y}F_y-byF_{by}\big)(byF_{by}-yF_y)}{y^2F_{yy}}h^{ii}(\partial_j\pi^j)
    -\tfrac12 a^4\tfrac{\left({y}^2 F_{yy} - {y}F_y\right)(byF_{by}-yF_y)}{y^2F_{yy}}h^{00}(\partial_j\pi^j)
    \\
    &\quad -\tfrac12 \tfrac{\big(2{y}F_y-byF_{by}\big)}{y^2F_{yy}}h^{ii}\bigg(\int\!d\tau(\partial_\ell\pi^\ell)\tfrac{d}{d\tau}(a^4yF_y)\bigg)
    -\tfrac12 \tfrac{\left({y}^2 F_{yy} - {y}F_y\right)}{y^2F_{yy}}h^{00}\bigg(\int\! d\tau(\partial_\ell\pi^\ell)\tfrac{d}{d\tau}(a^4yF_y)\bigg).
\end{aligned}
\end{align}}
Or equivalently keeping therms $\propto \, \nabla \pi+\int d\tau \nabla\pi$ together
{\small\color{red}
\begin{align}
\begin{aligned}
    -\tfrac12 a^4y^2F_{yy}\big(\dot{\pi}^0\big)^2
    &=-\tfrac{1}{2}\tfrac{a^4}{y^2F_{yy}}\bigg[(byF_{by}-yF_y) (\partial_j\pi^j)+\bigg(\tfrac{1}{a^4}\!\!\int\! d\tau\,(\partial_j \pi^j)\tfrac{d}{d\tau}(a^4yF_y)\bigg)\bigg]^2\\
    &\quad-\tfrac{a^4}{y^2F_{yy}}\Big[\big(2{y}F_y - byF_{by}\big) h^{ii}+ \left({y}^2 F_{yy} - {y}F_y\right) h^{00}\Big]\\
    &\qquad\qquad\cdot \bigg[(byF_{by}-yF_y) (\partial_j\pi^j)+\bigg(\tfrac{1}{a^4}\!\!\int\! d\tau\,(\partial_j \pi^j)\tfrac{d}{d\tau}(a^4yF_y)\bigg)\bigg]\,.
\end{aligned}
\end{align}}
%
Substituting back in the action we finally get\todotag{Rewrite w red exp, keeping $\nabla\pi+\int$ together}
{\small
\begin{align}
\begin{aligned}
    S^{(2)}=&\int d^4x\,\, a^4\,\frac{\rho+p}{2}\Bigg\{
    (\dot{\pi}^i)^2-\bigg[-\tfrac{b^2 F_{bb}}{(yF_y-bF_b)} +\tfrac{(byF_{by}-yF_y)^2}{y^2F_{yy}(yF_y-bF_b)}\bigg] (\partial_j \pi^j)^2 \\
    &\quad-2\tfrac{(byF_{by}-yF_y)}{y^2F_{yy}(yF_y-bF_b)} (\partial_j\pi^j)\bigg(\tfrac{1}{a^4}\int\!d\tau(\partial_\ell\pi^\ell)\tfrac{d}{d\tau}(a^4yF_y) \bigg)
    -\tfrac{1}{y^2F_{yy}(yF_y-bF_b)}\bigg(\tfrac{1}{a^4}\int(\partial_\ell\pi^\ell)\tfrac{d}{d\tau}(a^4yF_y)\bigg)^2\\
    &\quad +\left(\tfrac{\bar{b}F_b-\bar{b}^2 F_{bb}}{yF_y-bF_b} - \tfrac{\big(2{y}F_y-byF_{by}\big)(byF_{by}-yF_y)}{(yF_y-bF_b)y^2F_{yy}}\right) h^{ii}(\partial_j \pi^j)\\
    &\qquad\qquad\qquad+\!\left(\tfrac{\bar{b}\bar{y}F_{by}-2\bar{b}F_b}{yF_y-bF_b} - \tfrac{\left({y}^2 F_{yy} - {y}F_y\right)(byF_{by}-yF_y)}{(yF_y-bF_b)y^2F_{yy}}\right) h^{00}(\partial_j \pi^j)
    +2h^{0 j}\,\dot{\pi}^j\\
    &-\tfrac{\big(2{y}F_y-byF_{by}\big)}{y^2F_{yy}(yF_y-bF_b)}h^{ii}\bigg(\tfrac{1}{a^4}\int(\partial_\ell\pi^\ell)\tfrac{d}{d\tau}(a^4yF_y)\bigg)
    -\tfrac{\left({y}^2 F_{yy} - {y}F_y\right)}{y^2F_{yy}(yF_y-bF_b)}h^{00}\bigg(\tfrac{1}{a^4}\int(\partial_\ell\pi^\ell)\tfrac{d}{d\tau}(a^4yF_y)\bigg)\Bigg\}.
\end{aligned}
\end{align}}



